feat: extend type safety invariant to (ambient) traces.
In particular, this required slightly tweaking the type rules so that implicitly side-effecting ops (e.g., loadI) are only well-typed when the context is unrestricted. This does mean that some previously well-typed programs can no longer be typed. However, these are all programs where loadI/storeI occurs after createEff (and before the matching consumeEff). Recall that the semantics of createEff are that it consumes the ambient traces, and that loadI/storeI are UB when the ambient trace is missing. That is, all previously well-typed programs that are now excluded had UB, and thus excluding them is not a problem.

EffectSSA/Semantics/Typed/TProgram.lean
@@ -2,6 +2,7 @@ import EffectSSA.Syntax.Typed
 import EffectSSA.Semantics.Program
 import EffectSSA.Semantics.Lemmas
 import EffectSSA.Semantics.Typed.TEnvironment
+import EffectSSA.Semantics.Typed.TTrace
 
 /-!
 # Semantics of Intrinsically Typed Programs
@@ -29,25 +30,34 @@ theorem Instruction.isSome_exec {i : Instruction τ} {env : Environment τ}
   cases wt_i <;> (simp; (repeat rw [TEnvironment.env_getAs_eq (by assumption)]); try grind)
   next => simp
 
-def TInstruction.exec (i : TInstruction Γ Δ) (env : TEnvironment Γ) (es : Option (Trace τ)) :
-    TEnvironment Δ × (Option (Trace τ)) :=
-  let res := (i.instruction.exec env.env es).get <| Instruction.isSome_exec i.wt env.wt
-  have wt := by
+def TInstruction.exec (i : TInstruction Γ Δ) (env : TEnvironment Γ) (es : TTrace Γ) :
+    TEnvironment Δ × (TTrace Δ) :=
+  let res := (i.instruction.exec env.env es.get?).get <| Instruction.isSome_exec i.wt env.wt
+  have env_wt := by
     subst res
     cases i
     <;> (simp [Instruction.exec, Instruction.execM]; grind)
     -- TODO: Surely, this (^^) should be do-able without needing `simp` before `grind`
-  ⟨⟨res.1, wt⟩, res.2⟩
+  have trace_wt := by
+    subst res
+    cases i <;> (simp [Instruction.exec, Instruction.execM]; grind)
+  ⟨⟨res.1, env_wt⟩, ⟨res.2, trace_wt⟩⟩
 
 @[grind =>]
-theorem Instruction.exec_eq_of_wellTyped {i : Instruction τ} {env : Environment τ}
-    (wt_i : i.WellTyped Γ Δ) (wt_env : env.WellTyped Γ) (es?) :
-    i.exec env es? = some (TInstruction.exec ⟨i, wt_i⟩ ⟨env, wt_env⟩ es?) := by
+theorem Instruction.exec_eq_of_wellTyped {i : Instruction τ} {env : Environment τ} {es? : Option (Trace τ)}
+    (wt_i : i.WellTyped Γ Δ) (wt_env : env.WellTyped Γ) (wt_es?) :
+    i.exec env es? = some (
+      let r := TInstruction.exec ⟨i, wt_i⟩ ⟨env, wt_env⟩ ⟨es?, wt_es?⟩
+      (r.1.env, r.2.get?)
+    ) := by
   simp [TInstruction.exec]
 
 @[simp, grind =]
-theorem TInstruction.exec_instruction_eq {i : TInstruction Γ Δ} {env : TEnvironment Γ} :
-    i.instruction.exec env.env es? = some (i.exec env es?) := by
+theorem TInstruction.exec_instruction_eq {i : TInstruction Γ Δ} {env : TEnvironment Γ} (es : TTrace Γ) :
+    i.instruction.exec env.env es.get? = some (
+      let r := i.exec env es
+      (r.1.env, r.2.get?)
+    ) := by
   rw [Instruction.exec_eq_of_wellTyped]
 
 /-!
@@ -56,29 +66,38 @@ theorem TInstruction.exec_instruction_eq {i : TInstruction Γ Δ} {env : TEnviro
 
 @[grind! <=]
 theorem InstructionSeq.isSome_exec {is : InstructionSeq τ} {env : Environment τ}
-    (wt_is : is.WellTypedWith Γ Δ) (wt_env : env.WellTyped Γ) :
+    (wt_is : is.WellTypedWith Γ Δ) (wt_env : env.WellTyped Γ) (wt_es : Trace.WellTyped es Γ) :
     (is.exec env es).isSome := by
-  obtain ⟨env, rfl⟩ : ∃ (env' : TEnvironment _), env = env' := ⟨⟨env, wt_env⟩, rfl⟩
-  obtain ⟨is, rfl⟩ : ∃ (is' : TInstructionSeq _ _), is = is' := ⟨⟨is, wt_is⟩, rfl⟩
-  clear wt_env wt_is
-  induction is generalizing es <;> simp [*]
+  obtain ⟨env, rfl⟩ : ∃ (env' : TEnvironment _), env = env'.env := ⟨⟨env, wt_env⟩, rfl⟩
+  obtain ⟨is, rfl⟩ : ∃ (is' : TInstructionSeq _ _), is = is'.seq := ⟨⟨is, wt_is⟩, rfl⟩
+  obtain ⟨es, rfl⟩ : ∃ (es' : TTrace Γ), es = es'.get? := ⟨⟨es, wt_es⟩, rfl⟩
+  clear wt_env wt_is wt_es
+  induction is <;> simp [*]
 
-def TInstructionSeq.exec (is : TInstructionSeq Γ Δ) (env : TEnvironment Γ) (es? : Option (Trace τ)) :
-    TEnvironment Δ × Option (Trace τ) :=
-  let res := (is.seq.exec env es?).get <| InstructionSeq.isSome_exec is.wt env.wt
-  have wt := by intro v t; induction is generalizing es? <;> grind
-  ⟨⟨res.1, wt⟩, res.2⟩
+def TInstructionSeq.exec (is : TInstructionSeq Γ Δ) (env : TEnvironment Γ) (es? : TTrace Γ) :
+    TEnvironment Δ × TTrace Δ :=
+  let res := (is.seq.exec env es?).get <| InstructionSeq.isSome_exec is.wt env.wt es?.wt
+  have wt₁ := by intro v t; induction is <;> grind
+  have wt₂ := by induction is <;> grind
+  ⟨⟨res.1, wt₁⟩, ⟨res.2, wt₂⟩⟩
 
 
 @[grind =>]
-theorem InstructionSeq.exec_eq_of_wellTyped {is : InstructionSeq τ} {env : Environment τ}
-    (wt_i : is.WellTypedWith Γ Δ) (wt_env : env.WellTyped Γ) (es?) :
-    is.exec env es? = some (TInstructionSeq.exec ⟨is, wt_i⟩ ⟨env, wt_env⟩ es?) := by
+theorem InstructionSeq.exec_eq_of_wellTyped (wt_i : is.WellTypedWith Γ Δ)
+    (wt_env : env.WellTyped Γ) (wt_es? : Trace.WellTyped es? Γ) :
+    is.exec env es? = some (
+      let r := TInstructionSeq.exec ⟨is, wt_i⟩ ⟨env, wt_env⟩ ⟨es?, wt_es?⟩
+      (r.1.env, r.2.get?)
+    ) := by
   simp [TInstructionSeq.exec]
 
 @[simp, grind =]
-theorem TInstructionSeq.exec_instruction {is : TInstructionSeq Γ Δ} {env : TEnvironment Γ} :
-    is.seq.exec env.env es? = some (is.exec env es?) := by
+theorem TInstructionSeq.exec_instruction {is : TInstructionSeq Γ Δ} {env : TEnvironment Γ}
+    {es? : TTrace Γ}:
+    is.seq.exec env.env es?.get? = some (
+      let r := is.exec env es?
+      (r.1.env, r.2.get?)
+    ) := by
   rw [InstructionSeq.exec_eq_of_wellTyped]
 
 /-!
@@ -86,46 +105,60 @@ theorem TInstructionSeq.exec_instruction {is : TInstructionSeq Γ Δ} {env : TEn
 -/
 
 @[grind <=] theorem Program.isSome_exec {p : Program τ} {env : Environment τ}
-    (wt_p : p.WellTyped Γ ts) (wt_env : env.WellTyped Γ) :
+    (wt_p : p.WellTyped Γ ts) (wt_env : env.WellTyped Γ) (wt_es : Trace.WellTyped es Γ) :
     (p.exec env es).isSome := by
   obtain ⟨env, rfl⟩ : ∃ (env' : TEnvironment _), env = env' := ⟨⟨env, wt_env⟩, rfl⟩
   obtain ⟨p, rfl⟩ : ∃ (p' : TProgram _ _), p = p' := ⟨⟨p, wt_p⟩, rfl⟩
+  obtain ⟨es, rfl⟩ : ∃ (es' : TTrace Γ), es = es'.get? := ⟨⟨es, wt_es⟩, rfl⟩
   simp [exec, execM]
 
-def TProgram.exec (p : TProgram Γ ts) (env : TEnvironment Γ) (es? : Option (Trace τ)) :
-    TEnvironment ⟨ts⟩ × Option (Trace τ) :=
-  let res := (p.program.exec env es?).get <| Program.isSome_exec p.wt env.wt
-  have wt := by
-    simp [res, Environment.WellTyped, Program.exec, Program.execM]
-  ⟨⟨res.1, wt⟩, res.2⟩
+def TProgram.exec (p : TProgram Γ ts) (env : TEnvironment Γ) (es? : TTrace Γ) :
+    TEnvironment ⟨ts⟩ × TTrace ⟨ts⟩ :=
+  let res := (p.program.exec env es?).get <| Program.isSome_exec p.wt env.wt es?.wt
+  have wt₁ := by simp [res, Environment.WellTyped, Program.exec, Program.execM]
+  have wt₂ := by simp [res, Trace.WellTyped, Program.exec, Program.execM]
+  ⟨⟨res.1, wt₁⟩, ⟨res.2, wt₂⟩⟩
 
 @[grind] def TProgram.execClosed (p : TProgram (τ:=τ) ∅ ts) :
-    TEnvironment ⟨ts⟩ × Option (Trace τ) :=
-  p.exec ∅ (some ∅)
+    TEnvironment ⟨ts⟩ × TTrace ⟨ts⟩  :=
+  p.exec ∅ ∅
 
 section Lemmas
 
 @[grind =>]
 theorem Program.exec_eq_of_wellTyped {p : Program τ} {env : Environment τ}
-    (wt_p : p.WellTyped Γ ts) (wt_env : env.WellTyped Γ) (es?) :
-    p.exec env es? = some (TProgram.exec ⟨p, wt_p⟩ ⟨env, wt_env⟩ es? : Environment τ × _) := by
+    (wt_p : p.WellTyped Γ ts) (wt_env : env.WellTyped Γ) (wt_es? : Trace.WellTyped es? Γ) :
+    p.exec env es? = some (
+      let r := TProgram.exec ⟨p, wt_p⟩ ⟨env, wt_env⟩ ⟨es?, wt_es?⟩
+      (r.1.env, r.2.get?)
+    ) := by
   simp [TProgram.exec]
 
 @[simp, grind =]
-theorem TProgram.exec_program {p : TProgram Γ ts} {env : TEnvironment Γ} :
-    p.program.exec env.env es? = some (p.exec env es? : Environment τ × _) := by
-  simp [Program.exec_eq_of_wellTyped p.wt env.wt]
+theorem TProgram.exec_program {p : TProgram Γ ts} {env : TEnvironment Γ}
+    {es? : TTrace Γ}:
+    p.program.exec env.env es?.get? = some (
+      let r := p.exec env es?
+      (r.1.env, r.2.get?)
+    ) := by
+  simp [Program.exec_eq_of_wellTyped p.wt env.wt es?.wt]
 
 
 @[simp, grind =] theorem TProgram.execClosed_program {p : TProgram (τ:=τ) ∅ ts} :
-    p.program.execClosed = some (p.execClosed : Environment τ × _) := by
+    p.program.execClosed = some (
+      let r := p.execClosed
+      (r.1.env, r.2.get?)
+    ) := by
   have : (∅ : Environment τ) = (∅ : TEnvironment (τ:=τ) ∅) := rfl
-  simp only [Program.execClosed, this, TProgram.exec_program]
-  rfl
+  have : (some ∅ : Option (Trace τ)) = (∅ : TTrace (τ:=τ) ∅) := rfl
+  grind [Program.execClosed]
 
 @[simp] theorem Program.execClosed_eq_of_wellTyped {p : Program τ}
     (wt : p.WellTyped ∅ ts):
-    p.execClosed = some (TProgram.execClosed ⟨p, wt⟩ : Environment τ × _) := by
+    p.execClosed = some (
+      let r := TProgram.execClosed ⟨p, wt⟩
+      (r.1.env, r.2.get?)
+    ) := by
   generalize hp : TProgram.mk p wt = p'
   have : p = p'.program := by grind
   grind
