EffectSSA/Semantics/Typed/TTrace.lean
@@ -1,0 +1,75 @@
+import EffectSSA.Types
+import EffectSSA.Trace
+
+/-!
+# Intrinsically Typed Trace
+A program expects to be executed with an ambient trace iff its
+context is unrestricted, and it will return an ambient trace iff the returnTypes
+are unrestricted. Thus, we encode this into `TTrace Γ` intrinsically typed trace.
+-/
+namespace EffectSSA
+variable {τ} [MemorySignature τ]
+
+@[grind] def Trace.WellTyped (es? : Option (Trace τ)) (Γ : Context τ) : Prop :=
+  es?.isSome ↔ Γ.isUnrestricted
+
+/--
+`TTrace Γ` encodes an `Option (Trace τ)`, with the invariant that the trace
+is present iff `Γ` is unrestricted.
+-/
+structure TTrace (Γ : Context τ) where
+  get? : Option (Trace τ)
+  wt : Trace.WellTyped get? Γ := by grind
+
+/-!
+## Grind Lemmas
+--------------------------------------------------------------------------------
+-/
+namespace TTrace
+variable {Γ : Context τ}
+
+grind_pattern TTrace.wt => TTrace.get? self
+@[simp, grind = ] theorem get?_eq_none (es : TTrace Γ) : es.get? = none ↔ ¬Γ.isUnrestricted := by
+  grind [Option.not_isSome_iff_eq_none]
+
+
+/-!
+## Coercions
+--------------------------------------------------------------------------------
+-/
+variable {Γ : Context τ}
+
+instance : CoeOut (TTrace Γ) (Option (Trace τ)) where coe := TTrace.get?
+
+/-!
+## Definitions
+--------------------------------------------------------------------------------
+-/
+
+/--
+Retrieve the trace, given a proof that the context `Γ` is unrestricted.
+-/
+def get (t : TTrace Γ) (h : Γ.isUnrestricted := by grind) : Trace τ :=
+  t.get?.get (by grind)
+
+@[grind =] theorem get?_eq_none_of (t : TTrace Γ) (h : ¬Γ.isUnrestricted := by grind) :
+    t.get? = none := by
+  grind [Option.eq_none_of_isNone, Option.not_isSome]
+
+instance : EmptyCollection (TTrace (τ:=τ) ∅) where
+  emptyCollection := ⟨some ∅, by grind⟩
+
+/-- `missing` corresponds to a `none : Option (Trace τ)`. -/
+def missing (h : ¬Γ.isUnrestricted) : TTrace Γ where
+  get? := none
+
+/-!
+## Lemmas
+--------------------------------------------------------------------------------
+-/
+
+@[simp, grind =]
+theorem get?_isSome_eq (es : TTrace Γ) : es.get?.isSome = Γ.isUnrestricted := by grind
+
+@[simp, grind =]
+theorem get?_missing (h : ¬Γ.isUnrestricted) : get? (missing h) = none := by rfl
